Nflows case for low_proj_steps_implies_leq_step
This includes a proof of low_proj_steps_implies_leq_step for the case in
which a NodeStep is taken, and the particular node executing the step has a
label that is not visible to the observer. This was the case that seemed most
likely to determine whether or not the proof strategy will work
out, so the proof suggests it will.

Some new admitted theorems are introduced.

Some cleanup related to the placement of theorems was done.

experimental/ni_coq/vfiles/NIUtilTheorems.v
@@ -13,6 +13,136 @@ Import RecordSetNotations.
 
 Local Open Scope map_scope.
 
+Theorem eq_nodes_have_eq_lbls: forall n1 n2,
+    n1 = n2 -> (nlbl n1) = (nlbl n2).
+Proof. congruence. Qed.
+
+Theorem state_upd_node_eq: forall id n s,
+    (state_upd_node id n s).(nodes).[? id] = Some n.
+Proof.
+    intros. eapply upd_eq.
+Qed.
+
+Theorem state_upd_node_neq: forall (id id': node_id) n s,
+    id' <> id ->
+    (state_upd_node id n s).(nodes).[?id'] = s.(nodes).[?id'].
+Proof.
+    intros. eapply upd_neq. congruence.
+Qed.
+
+(*---------------------------------------------------------------------------*)
+(* Low Projections *)
+(*---------------------------------------------------------------------------*)
+Theorem flows_node_proj: forall ell n,
+    (nlbl n <<L ell) ->
+    (node_low_proj ell n) = n.
+Proof.
+    intros. unfold node_low_proj. destruct (nlbl n <<? ell). reflexivity.
+    contradiction.
+Qed.
+
+Theorem nflows_node_proj: forall ell n,
+    ~(nlbl n <<L ell) ->
+    (node_low_proj ell n) = (empty_node n.(nlbl)).
+Proof.
+    intros. unfold node_low_proj. destruct (nlbl n <<? ell). contradiction.
+    reflexivity.
+Qed.
+
+Theorem state_low_proj_idempotent: forall ell s,
+    (state_low_eq ell (state_low_proj ell s) s).
+Proof.
+Admitted.    
+
+Theorem state_low_proj_idempotent': forall ell s,
+    (state_low_proj ell (state_low_proj ell s)) = (state_low_proj ell s).
+Proof.
+Admitted.
+
+Theorem node_projection_preserves_lbl: forall ell n,
+    ((node_low_proj ell n).(nlbl) = n.(nlbl)).
+Proof.
+    intros. unfold node_low_proj. destruct (nlbl n <<? ell).
+    reflexivity. auto.
+Qed.
+
+Theorem proj_node_state_to_proj_n: forall ell s id n,
+    ((nodes (state_low_proj ell s)).[? id] = Some n) ->
+    exists n',
+        ((nodes s).[? id] = Some n') /\
+        (node_low_proj ell n') = n.
+Proof.
+    intros. 
+    unfold state_low_proj in H. cbn in H. unfold node_state_low_proj in H. cbn in H.
+    replace (nodes s id) with ((nodes s).[? id]) in H by reflexivity.
+    destruct ((nodes s).[? id]) eqn:Eidx.
+    - (* some *)
+    exists n0. split. reflexivity. congruence.
+    - (* none) *)
+    inversion H.
+Qed.
+
+Theorem node_projection_preserves_flowsto: forall ell s id n n',
+    s.(nodes).[? id] = Some n ->
+    (state_low_proj ell s).(nodes).[? id] = Some n' ->
+    ~(n.(nlbl) <<L ell) ->
+    ~(n'.(nlbl) <<L ell).
+Proof.
+    intros. unfold state_low_proj in *. cbn in H0.  unfold node_state_low_proj in H0.
+    destruct (nodes s id) eqn: E in H0. 
+        - (* some *) 
+        replace n0 with n in *.
+        erewrite nflows_node_proj in H0. inversion H0. auto. auto.
+        replace (nodes s id) with ((nodes s).[? id]) in E by auto.
+            (* why on earth do I need this, it's just notation ? *)
+            (* Do I need hint rewrites or something ? *)
+        congruence.
+        - (* none *)
+        inversion H0.
+Qed.
+
+(*---------------------------------------------------------------------------*)
+(* Low Equivalences *)
+(*---------------------------------------------------------------------------*)
+Definition transitive {A: Type} (r: A -> A -> Prop) :=
+        forall a1 a2 a3, (r a1 a2) -> (r a2 a3) -> (r a1 a3).
+
+Definition symmetric {A: Type} (r: A -> A -> Prop) := 
+    forall a1 a2, (r a1 a2) -> (r a2 a1).
+
+Theorem state_low_eq_trans: forall ell, transitive (state_low_eq ell).
+Proof.
+Admitted. (* WIP *)
+
+Theorem state_low_eq_sym: forall ell, symmetric (state_low_eq ell).
+Proof.
+Admitted. (* WIP *)
+
+Theorem event_low_eq_trans: forall ell, transitive (event_low_eq ell).
+Proof.
+Admitted. (* WIP *)
+
+Theorem state_loweq_to_deref_node: forall ell s1 s2 id n1,
+    (nodes s1).[? id] = Some n1 ->
+    (state_low_eq ell s1 s2) ->
+    exists n2,
+        (nodes s2).[? id] = Some n2 /\
+        (node_low_eq ell n1 n2).
+Proof.
+Admitted. (* WIP. For this one I think we need functional extensionality *)
+
+Theorem node_low_eq_to_lbl_eq: forall ell n1 n2,
+    (node_low_eq ell n1 n2) ->
+    (n1.(nlbl) = n2.(nlbl)).
+Proof.
+    intros. inversion H.
+    assert ( nlbl (node_low_proj ell n1) = nlbl (node_low_proj ell n2)).
+    rewrite H1. reflexivity.
+    rewrite node_projection_preserves_lbl in H0.
+    rewrite node_projection_preserves_lbl in H0.
+    assumption.
+Qed.
+
 Theorem trace_leq_imples_head_st_leq: forall ell t1 t2 s1 s2,
     (head_st t1 = Some s1) ->
     (head_st t2 = Some s2) ->
@@ -32,99 +162,6 @@ Proof.
             reflexivity. congruence.
         }
     congruence.
-Qed.
-
-Theorem flows_uncons_proj: forall ell n,
-    (nlbl n <<L ell) ->
-    (node_low_proj ell n) = n.
-Proof.
-    intros. unfold node_low_proj. destruct (nlbl n <<? ell). reflexivity.
-    contradiction.
-Qed.
-
-Theorem nflows_uncons_proj: forall ell n,
-    ~(nlbl n <<L ell) ->
-    (node_low_proj ell n) = (empty_node n.(nlbl)).
-Proof.
-    intros. unfold node_low_proj. destruct (nlbl n <<? ell). contradiction.
-    reflexivity.
-Qed.
-
-Theorem state_leq_and_flowsto_to_node_eq: forall ell s1 s2 id n1 n2,
-    (nodes s1).[? id] = Some n1 ->
-    (nodes s2).[? id] = Some n2 ->
-    (state_low_eq ell s1 s2) -> 
-    (nlbl n1 <<L ell) ->
-    n1 = n2.
-Proof.
-    (*
-    intros.
-    inversion H1. specialize (H3 id). rewrite H, H0 in H3. inversion H3.
-    assert (nlbl n2 <<L ell). destruct (nlbl n2 <<? ell).
-    assumption. rewrite flows_uncons_proj in H6. rewrite nflows_uncons_proj in H6.
-    *)
-Admitted.  (* WIP *)
-
-Theorem state_upd_chan_preserves_node_state_leq:
-    forall ell s1 s2 han1 ch1 han2 ch2,
-    node_state_low_eq ell (nodes s1) (nodes s2) ->
-    node_state_low_eq ell
-        (nodes (state_upd_chan han1 ch1 s1))
-        (nodes (state_upd_chan han2 ch2 s2)).
-Proof.
-Admitted. (* WIP // TODO *)
-
-Theorem state_upd_node_preserves_chan_state_leq:
-    forall ell s1 s2 id1 id2 n1 n2,
-    chan_state_low_eq ell (chans s1) (chans s2) ->
-    chan_state_low_eq ell
-        (chans (state_upd_node id1 n1 s1))
-        (chans (state_upd_node id2 n2 s2)).
-Proof.
-Admitted. (* WIP // TODO *)
-
-Theorem leq_node_updates_preserve_node_state_leq:
-    forall ell s1 s2 n1 n2 id,
-    node_state_low_eq ell (nodes s1) (nodes s2) ->
-    node_low_eq ell n1 n2 ->
-    node_state_low_eq ell
-        (nodes (state_upd_node id n1 s1)) (nodes (state_upd_node id n2 s2)).
-Proof.
-Admitted. (* WIP // TODO *)
-
-Theorem leq_chan_updates_preserve_chan_state_leq:
-    forall ell s1 s2 ch1 ch2 han,
-    chan_state_low_eq ell (chans s1) (chans s2) ->
-    chan_low_eq ell ch1 ch2 ->
-    chan_state_low_eq ell
-        (chans (state_upd_chan han ch1 s1)) (chans (state_upd_chan han ch2 s2)).
-Proof.
-Admitted. (* WIP // TODO *)
-
-Theorem node_low_eq_reflexive:
-    forall ell n, node_low_eq ell n n.
-Proof.
-Admitted. (* WIP // TODO *)
-
-Theorem other_chan_exists_from_chans_leq: forall ell s1 s2 han ch1,
-    chan_state_low_eq ell (chans s1) (chans s2) ->
-    (chans s1).[? han] = Some ch1 ->
-    exists ch2, ((chans s2).[? han ] = Some ch2) /\
-        (chan_low_eq ell ch1 ch2).
-Proof.
-Admitted. (* WIP // TODO *)
-
-Theorem state_upd_node_eq: forall id n s,
-    (state_upd_node id n s).(nodes).[? id] = Some n.
-Proof.
-    intros. eapply upd_eq.
-Qed.
-
-Theorem state_upd_node_neq: forall (id id': node_id) n s,
-    id' <> id ->
-    (state_upd_node id n s).(nodes).[?id'] = s.(nodes).[?id'].
-Proof.
-    intros. eapply upd_neq. congruence.
 Qed.
 
 Theorem trace_loweq_to_deref_node: forall ell t1 t2 id s1 n1,
@@ -167,3 +204,12 @@ Proof.
             + inversion Ht2head.
 Admitted. (* WIP *)
 
+(*---------------------------------------------------------------------------*)
+(* Unobservable *)
+(*---------------------------------------------------------------------------*)
+Theorem set_call_unobs: forall ell s id n c,
+    (nodes s).[? id] = Some n ->
+    ~(nlbl n <<L ell) ->
+    (state_low_eq ell s (s_set_call s id c)).
+Proof.
+Admitted. (* WIP *)
